Add simple lemmas to FreeVars and CAS

CAS.v
@@ -9,6 +9,64 @@ Inductive CAS : term -> id -> id -> term -> Prop :=
   | CAS_Var2 : forall x y z, z <> x -> CAS (Var z) x y (Var z)
   | CAS_App  : forall A B A' B' x y, CAS A x y A' -> CAS B x y B' -> CAS (App A B) x y (App A' B')
   | CAS_Lam1 : forall A x y, CAS (Lam x A) x y (Lam x A)
-  | CAS_Lam2 : forall A A' x y z, z <> x -> z <> y -> CAS A x y A' -> CAS (Lam z A) x y (Lam z A')
-  | CAS_Lam3 : forall A A' A'' x y z, not z ?? A -> CAS A y z A'' -> CAS A'' x y A' -> CAS (Lam y A) x y (Lam z A')
+  | CAS_Lam2 : forall A x y z, not x ?? A -> CAS (Lam z A) x y (Lam z A)
+  | CAS_Lam3 : forall A A' x y z, z <> x -> z <> y -> CAS A x y A' -> CAS (Lam z A) x y (Lam z A')
+  | CAS_Lam4 : forall A A' A'' x y z, not z ?? A -> CAS A y z A'' -> CAS A'' x y A' -> CAS (Lam y A) x y (Lam z A')
 .
+
+Hint Constructors CAS.
+
+Lemma CAS_same: forall A B x, CAS A x x B -> A = B.
+Proof.
+  intros.
+  admit.
+Admitted.
+
+Lemma CAS_other: forall A x y, not x ?? A -> not y ?? A -> CAS A x y A.
+Proof.
+  intros.
+  induction A.
+  - apply CAS_Var2.
+    apply FV_Var_other2 in H. auto.
+  - assert (not x ?? A1). { apply FV_App_not1 in H. auto. }
+    assert (not x ?? A2). { apply FV_App_not2 in H. auto. }
+    assert (not y ?? A1). { apply FV_App_not1 in H0. auto. }
+    assert (not y ?? A2). { apply FV_App_not2 in H0. auto. }
+    auto.
+  - destruct (eq_id_dec x i).
+    + subst. auto.
+    + destruct (eq_id_dec y i). subst.
+      * remember (CAS_Lam2 A x i i).
+        assert (not x ?? A). { remember (FV_Lam_body A x i). auto. }
+        auto.
+      * remember (CAS_Lam2 A x y i).
+        assert (not x ?? A). { remember (FV_Lam_body A x i). auto. }
+        auto.
+Qed.
+
+
+Lemma CAS_symm: forall A B x y, not y ?? A -> CAS A x y B -> CAS B y x A.
+Proof.
+    intros.
+    destruct (eq_id_dec x y).
+    subst. assert (A = B). { remember (CAS_same A B y). auto. }
+    subst. auto.
+    
+    induction A.
+    - inversion H0. subst.
+      + auto.
+      + subst. apply CAS_other.
+        destruct (eq_id_dec y i).
+        * subst. exfalso. apply FV_Var_other2 in H. auto.
+        * auto.
+        * apply FV_Var_other1. auto.
+    
+    - assert (not y ?? A1). { apply FV_App_not1 in H. auto. }
+      assert (not y ?? A2). { apply FV_App_not2 in H. auto. }
+      inversion H0.
+      subst.
+      admit.
+    - admit.
+Admitted.
+
+    
